\begin{activity}\label{A:0.4.2}
    Solve each of the following equations for $t$, and verify your answers using a calculator.
	\ba
		\item $\ln t=4$
		\item $\ln(t+3)=4$
		\item $\ln(t+3)=\ln4$
		\item $\ln(t+3)+\ln(t)=\ln4$
		\item $e^{t}=4$
		\item $e^{t+3}=4$
		\item $2e^{t+3}=4$
		\item $2e^{3t+2}=3e^{t-1}$
	\ea

\end{activity}
\begin{smallhint}
    
\end{smallhint}
\begin{bighint}
    
\end{bighint}
\begin{activitySolution}
    \ba
        \item $t = e^4$
        \item $t+3 = e^4$ so $t = e^4 - 3$
        \item $t+3 = 4$ so $t=1$
        \item Using the product property for logarithms, $\ln(t(t+3)) = \ln(4)$ so $t^2 +
            3t = 4$.  This is quadratic so we rearrange to get $t^2 + 3t - 4 = 0$ which
            factors to $(t+4)(t-1) = 0$ so the solutions are $t=1$ and $t=-4$.
            Substituting back to the original equation we see that $\ln(-4+3)$ and
            $\ln(-4)$ do not exist so the only solution is $t=1$.
        \item $t=\ln(4)$
        \item $t= \ln(4) = 3$
        \item $t+3 = \ln(2)$ so $t = \ln(2) = 3$
        \item For the final problem we first divide by $2$ and take the natural logarithm
            of both sides.
            \[ e^{3t+1} = \frac{3}{2} e^{t-1} \implies 3t+1 = \ln(3/2) + t-1. \]
            Therefore, $2t = \ln(3/2) - 2$ so $t=\frac{1}{2} \left( \ln(3/2) - 2 \right)$.
    \ea
\end{activitySolution}
\aftera
